Automata/Demos.lean
@@ -2,10 +2,11 @@ import Mathlib.Tactic
 import Automata.Equality
 import Automata.Addition
 import Automata.Projection
+import Automata.Boolean
+import Automata.ThueMorse
 
 theorem zero_is_zero : 0 = 0 := by
   apply (eqBase_iff_equal 2 (by norm_num) [0, 0] 2 (by norm_num) 0 1).mpr
-  unfold DFAO.eval DFAO.evalFrom
   native_decide
 
 
@@ -13,7 +14,6 @@ theorem foo : 100000 = 100000 := by
   apply (eqBase_iff_equal 2 (by norm_num) [100000, 100000] 2 (by norm_num) 0 1).mpr
   native_decide
 
--- What's difficult
 -- ∃ x, x = 0?
 #eval (project 0 (eqBase 2 2 0 1)).eval [fun _ => 0]
 
@@ -21,6 +21,9 @@ theorem foo : 100000 = 100000 := by
 #eval (project 2 (addBase 2)).eval [fun _ => 1]
 -- Wrong! Why? Projection only searches for representations in restricted length, 1+1 = 2 needs 2 bits.
 #eval (project 2 (addBase 2)).eval [fun _ => 0, fun _ => 1]
--- Correct after padding with 0s
-
+-- Correct with fixing leading zeros
 #eval (project 2 (addBase 2)).fixLeadingZeros.eval [fun _ => 1]
+
+-- ∃ x, t[x] = 0?
+#eval (project 0 (thueMorse.toDFA 0)).fixLeadingZeros.eval [fun _ => 0]
+
