Automata/ThueMorse.lean
@@ -6,12 +6,12 @@ import Automata.Input
 import Mathlib.Data.Nat.Digits
 
 
-def thueMorse : DFAO (Fin 2) (Fin 2) (Fin 2) := {
-  transition := fun a s => a + s
+def thueMorse : DFAO (Fin 1 → Fin 2) (Fin 2) (Fin 2) := {
+  transition := fun a s => a 0 + s
   start := 0
   output := fun x => x
 }
 
-def thueMorse0 : DFA (Fin 2) (Fin 2) := thueMorse.toDFA 0
+def thueMorse0 : DFA (Fin 1 → Fin 2) (Fin 2) := thueMorse.toDFA 0
 
-def thueMorse1 : DFA (Fin 2) (Fin 2) := thueMorse.toDFA 1
+def thueMorse1 : DFA (Fin 1 → Fin 2) (Fin 2) := thueMorse.toDFA 1
